\documentclass{article}
\usepackage {mathpartir}
\usepackage {amssymb}

\newcommand{\from}{\leftarrow}
\newcommand{\arr}{\rightarrow}
\newcommand{\kw}[1]{\mathtt{#1}}
\newcommand{\cc}{~::~}
\newcommand{\fun}{\star}

\newcommand{\eCase}[2]{\kw{case}~{#1}~\kw{of}~\{~{#2}~\}}
\newcommand{\eLetCase}[3]{\kw{case}~{#1}~\kw{of}~{#2}~\{~{#3}~\}}
\newcommand{\eLam}[2]{\lambda{#1}.~{#2}}
\newcommand{\eLet}[3]{\kw{let}~\{~{#1}={#2}~\}~\kw{in}~{#3}}
\newcommand{\eCut}[4]{\{ {#1} \from {#2}~|~{#3} \to {#4} \}}


\newcommand{\ju}[2]{\mathtt{#1} \cc {#2}}
\newcommand{\fits}[2]{{#1}\leftrightarrow{#2}}
\newcommand{\nofit}[2]{{#1}\nleftrightarrow{#2}}
\newcommand{\op}[1]{{#1}^\star}
\newcommand{\ty}[2]{\mathtt{#1}:{#2}}

\title{MALL}

\begin{document}

\section{Syntax}

\begin{mathpar}
t := s~|~\op s \\
s := a~|~()~|~(t,t)~|~0~|~(t+t) \\
\end{mathpar}

\section{No Proof Terms}

\begin{mathpar}

\infer
  {\fits a x}
  {a,x}

\infer
  {\fits a x}
  {a,x+p}

\infer
  {\fits a x}
  {a,p+x}

\infer
  { }
  {()}

\infer
  {\fits a x \\ \fits b y}
  {a,b,(x,y)}

\infer
  { }
  {\Gamma,\op 0}


\infer
  {\Gamma,a \\ \Delta,x \\ \fits a x}
  {\Gamma,\Delta}

\infer
  {\Gamma,x \\ \Gamma,y \\ \fits a x \\ \fits b y}
  {\Gamma,\op{(a+b)}}

\infer
  {\Gamma}
  {\Gamma,\op{()}}

\infer
  {\Gamma,x,y \\ \fits a x \\ \fits b y}
  {\Gamma,\op{(a,b)}}

\\

\infer
  { }
  {\fits a {\op a}}

\infer
  { }
  {\fits {\op a} a}
\end{mathpar}



\section{With Proof Terms}

The typing rules for an expression $e$ are of the form:
$$
\ju e \Gamma
$$

\begin{mathpar}

\infer
  {\fits a x}
  {\ju {u = v} {u:a, v:x}}

\infer
  {\fits a x}
  {\ju {u = L~v} {u:a+p, v:x}}

\infer
  {\fits a x}
  {\ju {u = R~v} {u:p+a, v:x}}

\infer
  { }
  {\ju {u = ()} {u:()}}

\infer
  {\fits a x \\ \fits b y}
  {\ju {u = (v,w)} {u:(x,y),v:a,w:b}}

\infer
  { }
  {\ju {u = \{ v_i \}} {u : \op 0, v_i:x_i}}


\infer
  {\ju {e1} {u:a,\Gamma} \\ \ju{e2} {v:x,\Delta} \\ \fits a x}
  {\ju{ \{ u \to e_1; v \to e_2 \}} {\Gamma,\Delta}}

\infer
  {\ju {e1} {v:x,\Gamma} \\ \ju {e2} {w:y,\Gamma} \\ \fits a x \\ \fits b y}
  {\ju {u = ~\{L~v \to e1; R~w \to~e2\}} {u:\op{(a+b)},\Gamma}}

\infer
  {\ju e {\Gamma}}
  {\ju {u = \{ () \to e \} } {u : \op{()}, \Gamma}}

\infer
  {\ju e {v:x,w:y,\Gamma} \\ \fits a x \\ \fits b y}
  {\ju {u = \{ (v,w) \to e \}} {u:\op{(a,b)},\Gamma}}

\end{mathpar}


\end{document}

